wip

examples/spinlock/spinlockScript.sml
@@ -444,7 +444,7 @@ Proof
 QED
 
 Theorem is_promise_is_fulfil:
-  !i j tr cid t. wf_trace tr /\ SUC i < LENGTH tr
+  !i tr cid t. wf_trace tr /\ SUC i < LENGTH tr
   /\ is_promise cid t (EL i tr) (EL (SUC i) tr)
   ==> ?j. i < j /\ SUC j < LENGTH tr
     /\ is_fulfil cid t (FST $ EL j tr) (FST $ EL (SUC j) tr)
@@ -501,7 +501,8 @@ QED
 Theorem wf_trace_EL_SND_is_promise:
   !i tr k. wf_trace tr /\ i < LENGTH tr
   /\ k < LENGTH $ SND $ EL i tr
-  ==> ?j. j < i /\ is_promise (EL k $ SND $ EL i tr).cid (SUC k) (EL j tr) (EL (SUC j) tr)
+  ==> ?j. j < i
+    /\ is_promise (EL k $ SND $ EL i tr).cid (SUC k) (EL j tr) (EL (SUC j) tr)
 Proof
   rpt strip_tac
   >> qmatch_goalsub_abbrev_tac `is_promise cid _ _`
@@ -622,15 +623,14 @@ Theorem is_fulfil_bst_coh:
   /\ FLOOKUP (FST $ EL j tr) cid = SOME $ Core cid p st
   ==> t < st.bst_coh((EL t $ SND $ EL (SUC i) tr).loc)
 Proof
-  ntac 3 gen_tac
+  rpt gen_tac
   >> Induct_on `j - i` >> fs[]
   >> rw[SUB_LEFT_EQ]
   >> first_x_assum $ qspecl_then [`v + i`,`i`] assume_tac
   >> Cases_on `0 < v`
   >> gs[]
   >- (
-    first_x_assum drule
-    >> cheat
+    cheat
   )
   >> drule_at_then (Pos $ el 3) assume_tac is_fulfil_parstep_nice_imp
   >> drule_at_then (Pos $ el 3) assume_tac is_fulfil_to_memory
@@ -648,6 +648,9 @@ Definition is_read_xcl_def:
     FLOOKUP sys1 cid = SOME $ Core cid p st
     /\ FLOOKUP sys2 cid = SOME $ Core cid p st'
     /\ bir_get_stmt p st.bst_pc = BirStmt_Read var a_e cast_opt T
+    /\ IS_SOME st'.bst_xclb
+    /\ (THE st'.bst_xclb).xclb_time = t
+    /\ IS_NONE st.bst_xclb
 End
 
 Definition is_fulfil_xcl_def:
@@ -679,6 +682,95 @@ Proof
   >> imp_res_tac is_fulfil_xcl_is_fulfil
   >> drule_at_then Any assume_tac is_fulfil_parstep_nice_eq
   >> gs[is_fulfil_xcl_def,bir_get_stmt_write]
+QED
+
+(* parstep and read transitions have same ids *)
+
+Theorem is_read_xcl_parstep_nice:
+  !tr i cid cid' t. wf_trace tr /\ SUC i < LENGTH tr
+  /\ is_read_xcl cid t (FST $ EL i tr) (FST $ EL (SUC i) tr)
+  /\ parstep_nice cid' (EL i tr) (EL (SUC i) tr)
+  ==> cid = cid'
+Proof
+  rpt strip_tac
+  >> `parstep_nice cid (EL i tr) (EL (SUC i) tr)` by (
+    CCONTR_TAC
+    >> fs[is_read_xcl_def]
+    >> drule_at Any wf_trace_NOT_parstep_nice_state_EQ'
+    >> rpt $ disch_then drule
+    >> disch_then $ fs o single
+  )
+  >> dxrule_at_then Any (drule_at Any) parstep_nice_parstep_nice
+  >> fs[]
+QED
+
+Theorem is_read_xcl_parstep_nice_imp:
+  !tr i cid t. wf_trace tr /\ SUC i < LENGTH tr
+  /\ is_read_xcl cid t (FST $ EL i tr) (FST $ EL (SUC i) tr)
+  ==> parstep_nice cid (EL i tr) (EL (SUC i) tr)
+Proof
+  rpt strip_tac
+  >> drule_all_then strip_assume_tac wf_trace_parstep_EL
+  >> drule_all is_read_xcl_parstep_nice
+  >> fs[]
+QED
+
+(* parstep transition of an exclusive read *)
+
+Theorem is_read_xcl_parstep_nice_eq:
+  !tr cid t i. wf_trace tr /\ SUC i < LENGTH tr
+    /\ is_read_xcl cid t (FST $ EL i tr) (FST $ EL (SUC i) tr)
+    ==> ?p s st' opt_cast ν_pre v_addr new_env l a_e var v.
+    is_certified p cid st' (SND (EL (SUC i) tr))
+    /\ st' = (s with
+           <|bst_pc := bir_pc_next (bir_pc_next s.bst_pc);
+             bst_environ := new_env;
+             bst_viewenv updated_by
+               (λenv.
+                    env |+
+                    (var,
+                     MAX (MAX v_addr s.bst_v_rNew)
+                       (mem_read_view a rk (s.bst_fwdb l) t)));
+             bst_coh :=
+               (λlo.
+                    if lo = l then
+                      MAX (s.bst_coh l)
+                        (MAX (MAX v_addr s.bst_v_rNew)
+                           (mem_read_view a rk (s.bst_fwdb l) t))
+                    else s.bst_coh lo);
+             bst_v_rOld :=
+               MAX s.bst_v_rOld
+                 (MAX (MAX v_addr s.bst_v_rNew)
+                    (mem_read_view a rk (s.bst_fwdb l) t));
+             bst_v_CAP := MAX s.bst_v_CAP v_addr;
+             bst_xclb :=
+               SOME
+                 <|xclb_time := t;
+                   xclb_view :=
+                     MAX (MAX v_addr s.bst_v_rNew)
+                       (mem_read_view a rk (s.bst_fwdb l) t)|> |>)
+    /\  SOME new_env =
+        env_update_cast64 (bir_var_name var) v (bir_var_type var) s.bst_environ
+    /\  (∀t'.
+          t < t' ∧ (t' ≤ ν_pre ∨ t' ≤ s.bst_coh l) ⇒
+          (EL t' (SND (EL i tr))).loc ≠ l)
+    /\  mem_read (SND (EL i tr)) l t = SOME v
+    /\  (SOME l,v_addr) = bir_eval_exp_view a_e s.bst_environ s.bst_viewenv
+    /\  bir_get_stmt p s.bst_pc = BirStmt_Read var a_e opt_cast T
+    /\  SND (EL (SUC i) tr) = SND (EL i tr)
+    /\  atomicity_ok cid (FST (EL i tr))
+    /\  FLOOKUP (FST (EL i tr)) cid = SOME (Core cid p s)
+    /\  FST (EL (SUC i) tr) = FST (EL i tr) |+ (cid, Core cid p st')
+Proof
+  rpt strip_tac
+  >> imp_res_tac is_read_xcl_parstep_nice_imp
+  >> dxrule_then assume_tac $ iffLR parstep_nice_def
+  >> dxrule_then strip_assume_tac $ iffLR parstep_cases
+  >> rpt $ goal_assum $ drule_at Any
+  >> gvs[cstep_cases,clstep_cases,is_read_xcl_def,optionTheory.IS_SOME_EXISTS,is_read_xcl_def,FLOOKUP_UPDATE]
+  >> rpt $ goal_assum $ drule_at Any
+  >> dsimp[bir_programTheory.bir_state_t_component_equality,pairTheory.ELIM_UNCURRY,FUN_EQ_THM,mem_read_view_def]
+  (* TODO remove free variables from definition mem_read_view_def *)
 QED
 
 (* only exclusive loads set the exclusive bank *)
@@ -725,6 +817,28 @@ Theorem is_fulfil_xcl_is_read_xcl:
       ==> st.bst_xclb = st'.bst_xclb
 Proof
   rpt strip_tac
+  >> drule_then assume_tac is_fulfil_xcl_is_fulfil
+  >> drule_all_then strip_assume_tac is_fulfil_is_promise
+  (* TODO there is a (last) process that sets the exclusive bank *)
+  >> qabbrev_tac `P = λj. 1 < j /\ LENGTH tr - j < i /\ j <= LENGTH tr
+    /\ !st st'. FLOOKUP (FST $ EL (LENGTH tr - j) tr) cid = SOME $ Core cid p st
+      /\ FLOOKUP (FST $ EL (SUC $ LENGTH tr - j) tr) cid = SOME $ Core cid p st'
+      ==> IS_NONE st.bst_xclb /\ IS_SOME st'.bst_xclb`
+  >> Cases_on `?i. P i`
+  >- (
+    dxrule_then assume_tac arithmeticTheory.WOP
+    >> fs[Abbr`P`,DISJ_EQ_IMP,AND_IMP_INTRO]
+    >> drule_then (drule_then $ qspec_then `LENGTH tr - n` assume_tac) wf_trace_cid
+    >> gs[]
+    >> cheat
+    >> `is_read_xcl cid t (FST (EL (LENGTH tr - n) tr)) (FST (EL (SUC $ LENGTH tr - n) tr))` by (
+      irule xclb_NONE_SOME_is_read_xclb
+      >> fs[]
+    )
+    >> goal_assum $ drule_at Any
+    (* TODO by xclb_NONE_SOME_is_read_xclb, this is an exclusive load *)
+    >> cheat
+  )
   >> cheat
 QED
 
@@ -736,12 +850,11 @@ Theorem varset_of_spinlock_prog =
   EVAL ``bir_varset_of_program $ bir_spinlock_prog:string bir_program_t``
 
 Definition spinlock_var_def:
-  spinlock_var = BExp_Den $ BVar "x7" $ BType_Imm Bit64
+  spinlock_var = BVar "x7" $ BType_Imm Bit64
 End
 
 Theorem spinlock_var_in_varset_of_spinlock_prog:
-  spinlock_var IN IMAGE BExp_Den $
-    bir_varset_of_program $ bir_spinlock_prog:string bir_program_t
+  spinlock_var IN bir_varset_of_program $ bir_spinlock_prog:string bir_program_t
 Proof
   fs[varset_of_spinlock_prog,spinlock_var_def]
 QED
@@ -819,7 +932,7 @@ Theorem bir_get_stmt_bir_spinlock_prog_BirStmt_Read_EQ:
   <=> st.bst_pc = <| bpc_index := 1; bpc_label := BL_Address $ Imm64 12w|>
     /\ var = BVar "x5" $ BType_Imm Bit64
     /\ opt_cast = SOME (BIExp_SignedCast,Bit64)
-    /\ a_e = spinlock_var
+    /\ a_e = BExp_Den spinlock_var
     /\ xcl
 Proof
   fs[EQ_IMP_THM]
@@ -844,12 +957,12 @@ Theorem bir_get_stmt_bir_spinlock_prog_BirStmt_Write_EQ:
   = BirStmt_Write a_e v_e xcl
   <=> (
     st.bst_pc = <| bpc_index := 2; bpc_label := BL_Address $ Imm64 12w|>
-    /\ a_e = spinlock_var
+    /\ a_e = BExp_Den spinlock_var
     /\ v_e = BExp_Const (Imm32 0x1010101w)
     /\ ~xcl
   ) \/ (
     st.bst_pc = <| bpc_index := 2; bpc_label := BL_Address $ Imm64 20w|>
-    /\ a_e = spinlock_var
+    /\ a_e = BExp_Den spinlock_var
     /\ v_e = BExp_Cast BIExp_LowCast (BExp_Den $ BVar "x0" $ BType_Imm Bit64) Bit32
     /\ xcl
   )
@@ -868,12 +981,14 @@ Proof
   >> fs[bir_get_stmt_write,bir_programTheory.bir_get_current_statement_def,CaseEq"option",pairTheory.ELIM_UNCURRY,spinlock_var_def,PULL_EXISTS,bir_get_program_block_info_by_label',get_fulfil_args_def,is_xcl_write_thm,bir_programTheory.bir_pc_next_def]
 QED
 
+(* an exclusive fulfil writes to the spinlock_var *)
+
 Theorem core_runs_spinlock_is_fulfil_xcl_memory_location:
   !tr i cid t p st. wf_trace tr /\ SUC i < LENGTH tr
   /\ core_runs_spinlock cid $ FST $ HD tr
   /\ is_fulfil_xcl cid t (FST $ EL i tr) (FST $ EL (SUC i) tr)
   /\ FLOOKUP (FST $ EL i tr) cid = SOME $ Core cid p st
-  ==> bir_eval_exp spinlock_var st.bst_environ
+  ==> bir_eval_exp (BExp_Den spinlock_var) st.bst_environ
     = SOME $ (EL (PRE t) $ SND $ EL i tr).loc
     /\ ?v. (EL (PRE t) $ SND $ EL i tr).val = BVal_Imm v
 Proof
@@ -896,7 +1011,97 @@ Proof
   >> fs[bir_expTheory.bir_eval_cast_def]
 QED
 
-(* Theorem 4 : any exclusive fulfil reads from timestamp 0 onwards *)
+(* the spinlock_var is 0w initially *)
+
+Theorem core_runs_spinlock_spinlock_var_default_value:
+  !tr i cid t p st x. wf_trace tr
+  /\ core_runs_spinlock cid $ FST $ HD tr
+  /\ FLOOKUP (FST $ HD tr) cid = SOME $ Core cid p st
+  /\ st.bst_environ = BEnv x
+  ==> x $ bir_var_name spinlock_var = SOME $ BVal_Imm $ Imm64 0w
+Proof
+  rpt gen_tac >> strip_tac
+  >> gvs[core_runs_spinlock_def,core_runs_prog_def,spinlock_var_def]
+  >> fs[bir_envTheory.bir_env_default_def,varset_of_spinlock_prog,bir_envTheory.bir_envty_of_vs_def]
+  >> dsimp[bir_envTheory.bir_var_name_def,bir_valuesTheory.bir_default_value_of_type_def,bir_envTheory.bir_var_type_def,bir_immTheory.n2bs_def]
+QED
+
+(* each exclusive read reads from a certain memory location *)
+(* TODO define the written value v *)
+Theorem core_runs_spinlock_is_read_xcl_memory_location:
+  !tr i cid t p st x. wf_trace tr /\ SUC i < LENGTH tr
+  /\ core_runs_spinlock cid $ FST $ HD tr
+  /\ is_read_xcl cid t (FST $ EL i tr) (FST $ EL (SUC i) tr)
+  /\ FLOOKUP (FST $ EL (SUC i) tr) cid = SOME $ Core cid p st
+  ==> bir_eval_exp (BExp_Den spinlock_var) st.bst_environ
+    = SOME $ (EL (PRE t) $ SND $ EL i tr).loc
+    /\ ?v. (EL (PRE t) $ SND $ EL i tr).val = BVal_Imm v
+Proof
+  cheat
+  (*
+  rpt gen_tac >> strip_tac
+  >> dxrule_at_then (Pat `is_fulfil _ _ _`) assume_tac is_read_parstep_nice_eq
+  >> drule_at Any wf_trace_core_runs_spinlock_FLOOKUP
+  >> disch_then $ drule_at_then Any assume_tac
+  >> gvs[is_fulfil_xcl_def,FLOOKUP_UPDATE,bir_get_stmt_bir_spinlock_prog_BirStmt_Write_EQ,bir_get_stmt_bir_spinlock_prog_BirStmt_Read_EQ]
+  >> qhdtm_x_assum `is_certified` kall_tac
+  >> qpat_x_assum `FST _ = _` kall_tac
+  >> fs[bir_expTheory.bir_eval_exp_def,bir_eval_exp_view_def,bir_envTheory.bir_env_read_def]
+  >> BasicProvers.every_case_tac
+  >> fs[bir_expTheory.bir_eval_cast_def,bir_envTheory.bir_env_lookup_type_def,bir_envTheory.bir_var_name_def]
+  >> qmatch_asmsub_rename_tac `bir_env_lookup "x0" st.bst_environ`
+  >> Cases_on `bir_env_lookup "x0" st.bst_environ`
+  >> gs[bir_expTheory.bir_eval_cast_def,bir_envTheory.bir_env_lookup_type_def,bir_envTheory.bir_var_name_def]
+  >> qmatch_asmsub_rename_tac `bir_eval_cast BIExp_LowCast (SOME x')`
+  >> Cases_on `x'`
+  >> fs[bir_expTheory.bir_eval_cast_def]
+  *)
+QED
+
+(* only one exclusive fulfil per thread can occur in a spinlock program *)
+
+Theorem core_runs_spinlock_is_fulfil_xcl_once:
+  !tr i j cid t t'. wf_trace tr /\ SUC i < LENGTH tr /\ SUC j < LENGTH tr
+  /\ core_runs_spinlock cid (FST $ HD tr)
+  /\ is_fulfil_xcl cid t (FST $ EL i tr) (FST $ EL (SUC i) tr)
+  /\ is_fulfil_xcl cid t' (FST $ EL j tr) (FST $ EL (SUC j) tr)
+  ==> t = t' /\ j = i
+Proof
+  rpt gen_tac >> strip_tac
+  >> conj_asm1_tac
+  >- cheat
+  >> spose_not_then assume_tac
+  >> imp_res_tac is_fulfil_xcl_is_fulfil
+  >> dxrule_at Any is_fulfil_once
+  >> fs[]
+  >> pop_assum $ irule_at Any
+  >> fs[]
+QED
+
+(* an exclusive fulfil reads the default value *)
+
+Theorem core_runs_spinlock_is_fulfil_xcl_is_read_xcl_default_value:
+  !tr cid t i j p st st'. wf_trace tr /\ SUC j < LENGTH tr
+  /\ core_runs_spinlock cid $ FST $ HD tr
+  /\ is_read_xcl cid t (FST $ EL i tr) (FST $ EL (SUC i) tr)
+  /\ is_fulfil_xcl cid t (FST $ EL j tr) (FST $ EL (SUC j) tr)
+  /\ i < j
+  /\ FLOOKUP (FST $ EL i tr) cid = SOME $ Core cid p st
+  /\ FLOOKUP (FST $ EL (SUC i) tr) cid = SOME $ Core cid p st'
+  ==> ?v. mem_read (SND $ EL i tr) ((EL (PRE t) (SND $ EL i tr)).loc) t
+          = SOME mem_default_value
+  /\ IS_SOME st'.bst_xclb /\ (THE st'.bst_xclb).xclb_time = 0
+Proof
+  rpt strip_tac
+  >> drule wf_trace_core_runs_spinlock_FLOOKUP
+  >> disch_then $ rev_drule_at_then (Pat `FLOOKUP _ _ = _`) assume_tac
+  >> drule_at_then (Pat `is_read_xcl _ _ _ _`) assume_tac is_read_xcl_parstep_nice_eq
+  >> gs[mem_read_view_def,optionTheory.IS_SOME_EXISTS,bir_programTheory.bir_state_t_component_equality,bir_programTheory.bir_state_t_accfupds]
+  >> imp_res_tac $ iffLR bir_get_stmt_bir_spinlock_prog_BirStmt_Read_EQ
+  >> cheat
+QED
+
+(* any exclusive fulfil reads from timestamp 0 onwards *)
 
 Theorem cores_run_spinlock_is_fulfil_xcl_initial_xclb:
   !tr cid t i s p st. wf_trace tr /\ SUC i < LENGTH tr
@@ -905,12 +1110,23 @@ Theorem cores_run_spinlock_is_fulfil_xcl_initial_xclb:
   /\ FLOOKUP (FST $ EL i tr) cid = SOME $ Core cid p st
   ==> IS_SOME st.bst_xclb /\ (THE st.bst_xclb).xclb_time = 0
 Proof
-  cheat
+  rpt gen_tac >> strip_tac
+  >> dxrule_at_then (Pat `is_fulfil_xcl _ _ _ _`) assume_tac is_fulfil_xcl_is_read_xcl
+  >> gvs[is_read_xcl_def]
+  >> drule wf_trace_core_runs_spinlock_FLOOKUP
+  >> disch_then $ rev_drule_at_then (Pat `FLOOKUP _ _ = _`) assume_tac
+  >> qmatch_assum_rename_tac `FLOOKUP (FST $ EL (SUC j) _) cid = _`
+  >> drule wf_trace_core_runs_spinlock_FLOOKUP
+  >> disch_then $ qspecl_then [`SUC j`,`cid`] assume_tac
+  >> first_x_assum $ qspec_then `SUC j` assume_tac
+  >> gvs[LESS_EQ,optionTheory.IS_SOME_EXISTS]
+  (* use core_runs_spinlock_is_fulfil_xcl_once *)
+  >> cheat
 QED
 
 (* any exiting core must have fulfiled exclusively *)
 
-Theorem core_runs_spinlock_IS_NONE_bst_pc_is_fulfil_xcl:
+Theorem core_runs_spinlock_bst_status_BST_JumpOutside_is_fulfil_xcl:
   !tr cid p st l. wf_trace tr
   /\ core_runs_spinlock cid (FST $ HD tr)
   /\ FLOOKUP (FST $ LAST tr) cid = SOME $ Core cid p st
@@ -925,15 +1141,108 @@ Proof
   >> cheat
 QED
 
+(* the address of the spinlock variable does not change *)
+
+Theorem core_runs_spinlock_memory_location_constant1:
+  !tr cid t i s p st st'. wf_trace tr /\ SUC i < LENGTH tr
+  /\ core_runs_spinlock cid $ FST $ HD tr
+  /\ FLOOKUP (FST $ EL i tr) cid = SOME $ Core cid p st
+  /\ FLOOKUP (FST $ EL (SUC i) tr) cid = SOME $ Core cid p st'
+  ==> bir_eval_exp (BExp_Den spinlock_var) st.bst_environ
+    = bir_eval_exp (BExp_Den spinlock_var) st'.bst_environ
+Proof
+  rpt strip_tac
+  >> drule_at Any wf_trace_core_runs_spinlock_FLOOKUP
+  >> drule_all wf_trace_parstep_EL
+  >> rw[]
+  >> qmatch_asmsub_rename_tac `parstep_nice cid'`
+  >> Cases_on `cid = cid'`
+  >> gvs[FLOOKUP_UPDATE,parstep_cases,parstep_nice_def]
+  >> gs[cstep_cases,FLOOKUP_UPDATE,clstep_cases]
+  >> qhdtm_x_assum `is_certified` kall_tac
+  >> qpat_x_assum `FST _ = _` kall_tac
+  >> gvs[]
+  >- (
+    (* BirStmt_Read *)
+    imp_res_tac $ iffLR bir_get_stmt_bir_spinlock_prog_BirStmt_Read_EQ
+    >> gvs[bir_eval_exp_view_def,bir_expTheory.bir_eval_exp_def,spinlock_var_def,bir_envTheory.bir_env_read_def,mem_read_def,mem_default_value_def,bir_envTheory.bir_env_update_def,bir_envTheory.bir_var_name_def]
+    >> Cases_on `t`
+    >> Cases_on `st.bst_environ`
+    >> gvs[env_update_cast64_def,bir_envTheory.bir_env_update_def,bir_envTheory.bir_env_lookup_def,FLOOKUP_UPDATE,bir_envTheory.bir_env_check_type_def,bir_envTheory.bir_env_lookup_type_def,bir_envTheory.bir_var_name_def,updateTheory.APPLY_UPDATE_THM,mem_read_def,mem_default_value_def,mem_read_aux_def]
+    >> qmatch_asmsub_rename_tac `mem_read_aux _ el`
+    >> Cases_on `el` >> fs[mem_read_aux_def,env_update_cast64_def]
+    >> cheat
+  )
+  >> Cases_on `s.bst_pc.bpc_index` >> fs[]
+  >> Cases_on `s.bst_pc.bpc_index < 5` >> gs[]
+  >> gs[LT5]
+  >> gvs[bir_eval_exp_view_def,bir_programTheory.bir_get_current_statement_def,CaseEq"option",pairTheory.ELIM_UNCURRY,bir_programTheory.bir_pc_next_def]
+  >> imp_res_tac $ REWRITE_RULE[optionTheory.IS_SOME_EXISTS] bir_spinlock_prog_labels
+  >> gs[bir_get_program_block_info_by_label',bir_programTheory.bir_pc_next_def]
+  >> gs[get_fulfil_args_def]
+  >> cheat
 (*
-TODO formulate theorem: (forward reasoning)
-any core running the spinlock can only have one is_fulfil_xcl transition
+bir_program_valid_stateTheory.bir_exec_stmtE_env_unchanged,
+bir_program_env_orderTheory.bir_exec_stmt_fence_SAME_ENV,
+bir_program_env_orderTheory.bir_exec_stmt_assume_SAME_ENV,
+bir_program_env_orderTheory.bir_exec_stmt_assert_SAME_ENV,
+bir_program_env_orderTheory.bir_exec_stmt_observe_SAME_ENV,
+bir_program_env_orderTheory.bir_state_set_failed_SAME_ENV,
+bir_program_valid_stateTheory.bir_exec_stmtE_env_unchanged,
+bir_programTheory.bir_state_t_accfupds
 *)
+QED
+
+(* any spinlock core only ever writes to the mutex variable memory location *)
+(* TODO set correct address k  *)
+Theorem cores_run_spinlock_is_fulfil_xcl_memory_location':
+  !tr cid t i s p st. wf_trace tr /\ SUC i < LENGTH tr
+  /\ core_runs_spinlock cid $ FST $ HD tr
+  /\ is_fulfil_xcl cid t (FST $ EL i tr) (FST $ EL (SUC i) tr)
+  ==> (EL (PRE t) $ SND $ EL i tr).loc = k
+    /\ (EL (PRE t) $ SND $ EL i tr).cid = cid
+Proof
+  rpt gen_tac >> strip_tac
+  >> imp_res_tac is_fulfil_xcl_is_fulfil
+  >> imp_res_tac is_fulfil_memory
+  >> dxrule_at_then (Pos $ el 3) assume_tac is_fulfil_parstep_nice_imp
+  >> dxrule_at_then (Pos $ el 3) assume_tac is_fulfil_xcl_atomic
+  >> gvs[is_fulfil_xcl_def,parstep_nice_def,parstep_cases,FLOOKUP_UPDATE,cstep_cases,clstep_cases,stmt_generic_step_def]
+  >> gs[]
+  >> cheat
+QED
+
+(* all spinlock cores write to the same location *)
+(* TODO set correct address k  *)
+Theorem cores_run_spinlock_unique_loc:
+  !tr i x. wf_trace tr /\ i < LENGTH tr
+  /\ cores_run_spinlock (FST $ HD tr)
+  /\ MEM x $ SND $ EL i tr
+  ==> x.loc = k
+Proof
+  rpt strip_tac
+  >> cheat
+  (*
+use thm core_runs_spinlock_is_fulfil_xcl_memory_location
+  >> Induct_on `LENGTH $ SND $ EL i tr`
+  >> rw[EVERY_MEM,MEM_EL]
+  >> Cases_on `i = 0`
+  >- (rw[] >> gvs[wf_trace_def,NULL_EQ])
+  >> qmatch_assum_rename_tac `i < LENGTH tr`
+  >> drule wf_trace_EL_SND_is_promise
+  >> rpt $ disch_then drule
+  >> drule_then (qspec_then `PRE i` assume_tac) wf_trace_parstep_EL
+  >> qmatch_asmsub_rename_tac `MEM x $ SND $ EL i tr`
+  >> gs[NOT_ZERO_LT_ZERO,AND_IMP_INTRO]
+  >> first_x_assum $ drule_at Any
+*)
+QED
 
 (* distinct exclusive fulfils enforce an ordering on their timestamps *)
 (* TODO replace "_xcl" assumptions with t and t' have same address *)
 Theorem core_runs_spinlock_is_fulfil_xcl_timestamp_order:
   !tr cid cid' t t' i j i' j'. wf_trace tr
+  /\ cores_run_spinlock (FST $ HD tr)
   /\ core_runs_spinlock cid (FST $ HD tr)
   /\ core_runs_spinlock cid' (FST $ HD tr)
   /\ is_fulfil_xcl cid t (FST $ EL i tr) (FST $ EL (SUC i) tr)
@@ -944,11 +1253,55 @@ Theorem core_runs_spinlock_is_fulfil_xcl_timestamp_order:
   ==> ~(t < t')
 Proof
   rpt strip_tac
+  >> `cid <> cid'` by (
+    spose_not_then assume_tac
+    >> gvs[]
+    >> dxrule core_runs_spinlock_is_fulfil_xcl_once
+    >> rpt $ disch_then $ dxrule_at Any
+    >> fs[]
+  )
   >> drule_at_then (Pos $ el 4) assume_tac cores_run_spinlock_is_fulfil_xcl_initial_xclb
   >> rev_drule_at_then (Pos $ el 4) assume_tac cores_run_spinlock_is_fulfil_xcl_initial_xclb
-  >> gs[is_fulfil_xcl_def]
+  >> drule_at_then (Pat `is_fulfil_xcl _ _ _ _`) assume_tac is_fulfil_xcl_atomic
+  >> rev_drule_at_then (Pat `is_fulfil_xcl _ _ _ _`) assume_tac is_fulfil_xcl_atomic
+  >> imp_res_tac is_fulfil_xcl_is_fulfil
+  >> gs[is_fulfil_xcl_def,optionTheory.IS_SOME_EXISTS]
+  >> rev_drule_at_then (Pat `FLOOKUP _ _ = _`) assume_tac wf_trace_core_runs_spinlock_FLOOKUP
+  >> drule_at_then (Pat `FLOOKUP _ _ = _`) assume_tac wf_trace_core_runs_spinlock_FLOOKUP
+  >> gvs[bir_get_stmt_bir_spinlock_prog_BirStmt_Write_EQ]
+  >> qmatch_assum_rename_tac `fulfil_atomic_ok (SND $ EL i' tr) _ cid' _ t'`
+  >> qmatch_assum_rename_tac `fulfil_atomic_ok (SND $ EL i tr) _ cid _ t`
+  >> `(EL (PRE t) (SND $ EL i tr)).loc = k /\ (EL (PRE t') (SND $ EL i' tr)).loc = k` by (
+    ntac 2 $ dxrule_at_then (Pat `is_fulfil _ _ _ _`) assume_tac is_fulfil_to_memory
+    >> drule cores_run_spinlock_unique_loc
+    >> disch_then $ (fn x =>
+      qspecl_then [`k`,`i'`,`EL (PRE t') $ SND $ EL i' tr`] assume_tac x
+      >> qspecl_then [`k`,`i`,`EL (PRE t) $ SND $ EL i tr`] assume_tac x
+    )
+    >> gvs[EL_MEM]
+  )
+  >> drule cores_run_spinlock_unique_loc
+  >> disch_then $ (fn x =>
+    qspecl_then [`k`,`i'`,`HD $ SND $ EL i' tr`] assume_tac x
+    >> qspecl_then [`k`,`i`,`HD $ SND $ EL i tr`] assume_tac x
+  )
+  >> drule_at_then (Pat `is_fulfil _ _ _ _`) assume_tac is_fulfil_to_memory
+  >> rev_drule_at_then (Pat `is_fulfil _ _ _ _`) assume_tac is_fulfil_to_memory
   (* contradiction with atomic predicate and exclusivity bank *)
-  >> cheat
+  >> `0 < LENGTH $ SND $ EL i' tr /\ 0 < LENGTH $ SND $ EL i tr` by (
+    fs[is_promise_def]
+    >> drule wf_trace_IS_PREFIX_SND_EL
+    >> disch_then $ (fn x =>
+      qspecl_then [`SUC j`,`SUC i`] assume_tac x
+      >> qspecl_then [`SUC j'`,`SUC i'`] assume_tac x
+    )
+    >> gs[IS_PREFIX_APPEND]
+    >> cheat (* minor *)
+  )
+  >> gs[fulfil_atomic_ok_def,Excl"EL",GSYM EL,Excl"EL_restricted",EL_MEM]
+  >> last_x_assum $ qspec_then `t` assume_tac
+  >> gs[GSYM PRE_SUB1]
+  >> cheat (* minor *)
 QED
 
 (* Theorem 5 only one core can leave the lock region *)
@@ -965,9 +1318,9 @@ Theorem core_runs_spinlock_correct:
 Proof
   rpt strip_tac
   >> drule_then assume_tac wf_trace_NOT_NULL
-  >> drule_then drule core_runs_spinlock_IS_NONE_bst_pc_is_fulfil_xcl
+  >> drule_then drule core_runs_spinlock_bst_status_BST_JumpOutside_is_fulfil_xcl
   >> rpt $ disch_then $ dxrule
-  >> drule_then rev_drule core_runs_spinlock_IS_NONE_bst_pc_is_fulfil_xcl
+  >> drule_then rev_drule core_runs_spinlock_bst_status_BST_JumpOutside_is_fulfil_xcl
   >> rpt $ disch_then $ dxrule
   >> rw[]
   >> imp_res_tac is_fulfil_xcl_is_fulfil
@@ -997,16 +1350,13 @@ Proof
     >> rpt $ disch_then dxrule
     >> fs[]
   )
-  >> `~(t < t')` by (
-    drule_then rev_drule core_runs_spinlock_is_fulfil_xcl_timestamp_order
-    >> rpt $ disch_then drule
-    >> fs[]
-  )
-  >> `~(t' < t)` by (
-    drule_then drule core_runs_spinlock_is_fulfil_xcl_timestamp_order
-    >> rpt $ disch_then rev_drule
-    >> fs[]
-  )
+  >> drule_then drule core_runs_spinlock_is_fulfil_xcl_timestamp_order
+  >> disch_then $ rev_drule
+  >> rpt $ disch_then $ drule
+  >> drule_then drule core_runs_spinlock_is_fulfil_xcl_timestamp_order
+  >> disch_then $ drule
+  >> disch_then $ rev_drule
+  >> rpt $ disch_then $ drule
   >> fs[]
 QED
 
